Weidenbach_Book/Watched_Literals_Watch_List_Domain.thy
@@ -19,6 +19,7 @@ type_synonym clause_wl = \<open>uint32 array\<close>
 type_synonym unit_lits_wl = \<open>uint32 list list\<close>
 
 type_synonym watched_wl = \<open>(nat array_list) array\<close>
+type_synonym watched_wl_uint32 = \<open>(uint32 array_list) array\<close>
 
 
 subsubsection \<open>Refinement of the Watched Function\<close>
@@ -146,7 +147,8 @@ definition ann_lit_rel:: \<open>('a \<times> nat) set \<Rightarrow> ('b \<times>
 
 type_synonym ann_lit_wl = \<open>uint32 \<times> nat option\<close>
 type_synonym ann_lits_wl = \<open>ann_lit_wl list\<close>
-term \<open> \<langle>uint32_nat_rel\<rangle>option_rel\<close>
+type_synonym ann_lit_wl_fast = \<open>uint32 \<times> uint32 option\<close>
+type_synonym ann_lits_wl_fast = \<open>ann_lit_wl_fast list\<close>
 
 definition nat_ann_lit_rel :: \<open>(ann_lit_wl \<times> (nat, nat) ann_lit) set\<close> where
   nat_ann_lit_rel_internal_def: \<open>nat_ann_lit_rel = \<langle>uint32_nat_rel, \<langle>nat_rel\<rangle>option_rel\<rangle>ann_lit_rel\<close>
@@ -174,6 +176,12 @@ abbreviation pair_nat_ann_lit_assn :: \<open>(nat, nat) ann_lit \<Rightarrow> an
 
 abbreviation pair_nat_ann_lits_assn :: \<open>(nat, nat) ann_lits \<Rightarrow> ann_lits_wl \<Rightarrow> assn\<close> where
   \<open>pair_nat_ann_lits_assn \<equiv> list_assn pair_nat_ann_lit_assn\<close>
+
+abbreviation pair_nat_ann_lit_fast_assn :: \<open>(nat, nat) ann_lit \<Rightarrow> ann_lit_wl_fast \<Rightarrow> assn\<close> where
+  \<open>pair_nat_ann_lit_fast_assn \<equiv> hr_comp (uint32_assn *a option_assn uint32_nat_assn) nat_ann_lit_rel\<close>
+
+abbreviation pair_nat_ann_lits_fast_assn :: \<open>(nat, nat) ann_lits \<Rightarrow> ann_lits_wl_fast \<Rightarrow> assn\<close> where
+  \<open>pair_nat_ann_lits_fast_assn \<equiv> list_assn pair_nat_ann_lit_fast_assn\<close>
 
 lemma nat_ann_lits_rel_Cons[iff]:
   \<open>(x # xs, y # ys) \<in> nat_ann_lits_rel \<longleftrightarrow> (x, y) \<in> nat_ann_lit_rel \<and> (xs, ys) \<in> nat_ann_lits_rel\<close>
@@ -1751,6 +1759,65 @@ proof -
       subgoal using T by fast
       subgoal unfolding conc_fun_chain by (rule conc_fun_R_mono) blast
       done
+    done
+qed
+
+
+definition (in isasat_input_ops) cdcl_twl_stgy_prog_break_wl_D
+   :: \<open>nat twl_st_wl \<Rightarrow> nat twl_st_wl nres\<close>
+where
+  \<open>cdcl_twl_stgy_prog_break_wl_D S\<^sub>0 =
+  do {
+    b \<leftarrow> SPEC(\<lambda>_. True);
+    (b, brk, T) \<leftarrow> WHILE\<^sub>T\<^bsup>\<lambda>(b, brk, T). cdcl_twl_stgy_prog_wl_inv S\<^sub>0 (brk, T)\<and>
+          literals_are_\<L>\<^sub>i\<^sub>n T\<^esup>
+        (\<lambda>(b, brk, _). b \<and> \<not>brk)
+        (\<lambda>(b, brk, S).
+        do {
+          T \<leftarrow> unit_propagation_outer_loop_wl_D S;
+          T \<leftarrow> cdcl_twl_o_prog_wl_D T;
+          b \<leftarrow> SPEC(\<lambda>_. True);
+          RETURN(b, T)
+        })
+        (b, False, S\<^sub>0);
+    if brk then RETURN T
+    else cdcl_twl_stgy_prog_wl_D T
+  }\<close>
+
+theorem cdcl_twl_stgy_prog_break_wl_D_spec:
+  assumes \<open>literals_are_\<L>\<^sub>i\<^sub>n S\<close>
+  shows \<open>cdcl_twl_stgy_prog_break_wl_D S \<le> \<Down> {(T', T). T = T' \<and> literals_are_\<L>\<^sub>i\<^sub>n T}
+     (cdcl_twl_stgy_prog_break_wl S)\<close>
+proof -
+  have 1: \<open>((b, False, S), b, False, S) \<in> {((b', brk', T'), b, brk, T). b = b' \<and> brk = brk' \<and>
+        T = T' \<and> literals_are_\<L>\<^sub>i\<^sub>n T}\<close>
+    for b
+    using assms by fast
+  have 1: \<open>((b, False, S), b', False, S) \<in> {((b', brk', T'), b, brk, T). b = b' \<and> brk = brk' \<and>
+        T = T' \<and> literals_are_\<L>\<^sub>i\<^sub>n T}\<close>
+    if \<open>(b, b') \<in> bool_rel\<close> 
+    for b b'
+    using assms that by fast
+  have 2: \<open>unit_propagation_outer_loop_wl_D S \<le> \<Down> {(T', T). T = T' \<and> literals_are_\<L>\<^sub>i\<^sub>n T}
+       (unit_propagation_outer_loop_wl T)\<close> if \<open>S = T\<close> \<open>literals_are_\<L>\<^sub>i\<^sub>n S\<close> for S T
+    using unit_propagation_outer_loop_wl_D_spec[of S] that by fast
+  have 3: \<open>cdcl_twl_o_prog_wl_D S \<le> \<Down> {((b', T'), b, T). b = b' \<and> T = T' \<and> literals_are_\<L>\<^sub>i\<^sub>n T}
+    (cdcl_twl_o_prog_wl T)\<close> if \<open>S = T\<close> \<open>literals_are_\<L>\<^sub>i\<^sub>n S\<close> for S T
+    using cdcl_twl_o_prog_wl_D_spec[of S] that by fast
+  show ?thesis
+    unfolding cdcl_twl_stgy_prog_break_wl_D_def cdcl_twl_stgy_prog_break_wl_def
+    apply (refine_vcg 1 2 3)
+    subgoal by fast
+    subgoal by fast
+    subgoal by fast
+    subgoal by fast
+    subgoal by fast
+    subgoal by fast
+    subgoal by fast
+    subgoal by fast
+    subgoal by fast
+    subgoal by fast
+    subgoal by (fast intro!: cdcl_twl_stgy_prog_wl_D_spec)
     done
 qed
 
